Progress on adding physical actions

src/ReactorModel/Execution/Basic.lean
@@ -11,7 +11,7 @@ inductive Apply : Change → State α → State α → Type
   | inp {rtr} : (LawfulUpdate .inp i v s.rtr rtr) → Apply (.inp i v) s { s with rtr }    
   | out {rtr} : (LawfulUpdate .out i v s.rtr rtr) → Apply (.out i v) s { s with rtr }    
   | stv {rtr} : (LawfulUpdate .stv i v s.rtr rtr) → Apply (.stv i v) s { s with rtr }    
-  | act : Apply (.act i t v ) s (s.schedule i t v)
+  | act : Apply (.act i t v ) s (s.schedule .log i t v)
   | mut : Apply (.mut _) s s -- Mutations are currently no-ops.
   
 notation s₁:max " -[" c "]→ " s₂:max => Apply c s₁ s₂
@@ -23,20 +23,26 @@ inductive Apply.RTC : Reaction.Output → State α → State α → Type
 notation s₁:max " -[" cs "]→ " s₂:max => Apply.RTC cs s₁ s₂
 
 inductive Skip : State α → State α → Type
-  | mk : (Allows s rcn) → (¬Triggers s rcn) → Skip s (s.record rcn)
+  | mk : (Allows s rcn) → (¬Triggers s rcn) → (s.clock ≤ t) → Skip s (s.at t |>.record rcn)
 
 notation s₁:max " ↓ₛ " s₂:max => Skip s₁ s₂
 
 inductive Exec : State α → State α → Type
-  | mk : (Allows s₁ rcn) → (Triggers s₁ rcn) → (s₁ -[s₁.output rcn]→ s₂) → Exec s₁ (s₂.record rcn)
+  | mk : (Allows s₁ rcn) → (Triggers s₁ rcn) → (s₁ -[s₁.output rcn]→ s₂) → (s₁.clock ≤ t) → 
+         Exec s₁ (s₂.at t |>.record rcn)
 
 notation s₁:max " ↓ₑ " s₂:max => Exec s₁ s₂
 
 inductive Time : State α → State α → Type
-  | mk : (Closed s) → (NextTag s g) → (Refresh s.rtr ref $ s.logicals g) → 
-         Time s { s with rtr := ref, tag := g, progress := ∅ }
+  | mk : (Closed s) → (NextTag s g) → (Refresh s.rtr ref $ s.logicals g) → (g.time ≤ t) → 
+         Time s { s with rtr := ref, tag := g, clock := t, progress := ∅ }
 
 notation s₁:max " ↓ₜ " s₂:max => Time s₁ s₂
+
+inductive Phys : State α → State α → Type
+  | mk {phy : ID} : Phys s s -- TODO
+
+notation s₁:max " ↓ₚ " s₂:max => Exec s₁ s₂
 
 end Step
 
@@ -44,6 +50,7 @@ inductive Step (s₁ s₂ : State α) : Prop
   | skip (s : s₁ ↓ₛ s₂)
   | exec (e : s₁ ↓ₑ s₂)
   | time (t : s₁ ↓ₜ s₂)
+  | phys (p : s₁ ↓ₚ s₂)
 
 notation s₁:max " ↓ " s₂:max => Step s₁ s₂
 
