src/lakefile.lean
@@ -5,8 +5,8 @@ package reactor_model
 
 lean_lib ReactorModel
 
-require mathlib from git "https://github.com/leanprover-community/mathlib4.git"@"d2b5332904d3d3b874"
+require mathlib from git "https://github.com/leanprover-community/mathlib4.git"@"0285b69b1fd0fa0f63"
 
 -- https://github.com/leanprover/doc-gen4#usage
-meta if get_config? env = some "dev" then 
-require «doc-gen4» from git "https://github.com/leanprover/doc-gen4"@"master"
+-- meta if get_config? env = some "dev" then 
+-- require «doc-gen4» from git "https://github.com/leanprover/doc-gen4"@"master"
